Define fulfill step and prove lemmas

src/promising/PFRel.v
@@ -27,6 +27,53 @@ Set Implicit Arguments.
 Set Nested Proofs Allowed.
 
 
+Definition promises_eq_until (n: Time.t) (p1 p2: Promises.t): Prop :=
+  forall ts (LE: ts <= n), Promises.lookup ts p1 = Promises.lookup ts p2.
+
+Program Instance promises_eq_until_Equivalence (n: Time.t): Equivalence (promises_eq_until n).
+Next Obligation.
+  ii. ss.
+Qed.
+Next Obligation.
+  ii. rewrite H; ss.
+Qed.
+Next Obligation.
+  ii. rewrite H, H0; ss.
+Qed.
+
+Lemma promises_eq_until_decr
+      n m p1 p2
+      (LE: m <= n)
+      (EQ: promises_eq_until n p1 p2):
+  promises_eq_until m p1 p2.
+Proof.
+  ii. rewrite EQ; ss. nia.
+Qed.
+
+Definition promises_sound (tid: Id.t) (prm: Promises.t) (mem: Memory.t): Prop :=
+  forall ts (LOOKUP: Promises.lookup ts prm),
+  exists msg,
+    (<<GET: Memory.get_msg ts mem = Some msg>>) /\
+    (<<TID: msg.(Msg.tid) = tid>>).
+
+Lemma le_promises_sound
+      tid prm1 prm2 mem
+      (SOUND: promises_sound tid prm1 mem)
+      (LE: Promises.le prm2 prm1):
+  promises_sound tid prm2 mem.
+Proof.
+  ii. eauto.
+Qed.
+
+Definition is_release {A} `{_: orderC A} (e: Event.t (A:=A)): bool :=
+  match e with
+  | Event.write _ ordw _ _ _
+  | Event.fadd _ ordw _ _ _ => OrdW.ge OrdW.release_pc ordw
+  | Event.barrier (Barrier.dmb rr rw wr ww) => andb rw ww
+  | _ => false
+  end.
+
+
 Module PFRelLocal.
   Section PFRelLocal.
     Import Local.
@@ -91,6 +138,55 @@ Module PFRelLocal.
     .
     #[local]
      Hint Constructors step: core.
+
+    Lemma step_promises_le
+          e tid lc1 mem1 lc2 mem2
+          (STEP: step e tid lc1 mem1 lc2 mem2):
+      Promises.le (promises lc2) (promises lc1).
+    Proof.
+      inv STEP; ss; try by (inv STEP0; ss).
+      - inv STEP0. ss. apply Promises.unset_le.
+      - inv STEP_PROMISE. inv STEP_FULFILL. ss.
+        apply Promises.unset_set_le.
+      - inv STEP_READ. inv STEP_FULFILL. ss.
+        apply Promises.unset_le.
+      - inv STEP_READ. inv STEP_PROMISE. ss. inv STEP_FULFILL. ss.
+        apply Promises.unset_set_le.
+      - inv LC. ss.
+    Qed.
+
+    Variant more_promises (n: Time.t) (lc1 lc2: t (A:=A)): Prop :=
+    | more_promises_intro
+        (COH: coh lc1 = coh lc2)
+        (VRN: vrn lc1 = vrn lc2)
+        (VWN: vwn lc1 = vwn lc2)
+        (VRO: vro lc1 = vro lc2)
+        (VWO: vwo lc1 = vwo lc2)
+        (VCAP: vcap lc1 = vcap lc2)
+        (VREL: vrel lc1 = vrel lc2)
+        (FWDBANK: fwdbank lc1 = fwdbank lc2)
+        (EXBANK: exbank lc1 = exbank lc2)
+        (PROMISES_LE: Promises.le (promises lc1) (promises lc2))
+        (PROMISES_EQ: promises_eq_until n (promises lc1) (promises lc2))
+    .
+
+    Global Program Instance more_promises_PreOrder n: PreOrder (more_promises n).
+    Next Obligation.
+      ii. econs; ss.
+    Qed.
+    Next Obligation.
+      ii. inv H1. inv H2.
+      econs; try congr; etrans; eauto.
+    Qed.
+
+    Lemma more_promises_decr
+          m n lc1 lc2
+          (MORE: more_promises n lc1 lc2)
+          (MN: m <= n):
+      more_promises m lc1 lc2.
+    Proof.
+      inv MORE. econs; eauto using promises_eq_until_decr.
+    Qed.
   End PFRelLocal.
 End PFRelLocal.
 
@@ -122,6 +218,40 @@ Module PFRelExecUnit.
     .
     #[local]
      Hint Constructors step: core.
+
+    Variant non_rel_step (tid:Id.t) (eu1 eu2:t): Prop :=
+    | non_rel_step_intro
+        e
+        (STEP: ExecUnit.state_step0 tid e e eu1 eu2)
+        (REL: ~ is_release e)
+    .
+    #[local]
+     Hint Constructors non_rel_step: core.
+
+    Variant rel_step (tid:Id.t) (eu1 eu2:t): Prop :=
+    | rel_step_intro
+        e
+        (STEP: ExecUnit.state_step0 tid e e eu1 eu2)
+        (REL: is_release e)
+    .
+    #[local]
+     Hint Constructors rel_step: core.
+
+    Variant fulfilled (ts: Time.t) (eu1 eu2: t): Prop :=
+    | fulfilled_intro
+        (BEFORE: Promises.lookup ts eu1.(ExecUnit.local).(Local.promises))
+        (AFTER: ~ Promises.lookup ts eu2.(ExecUnit.local).(Local.promises))
+    .
+    #[local]
+     Hint Constructors fulfilled: core.
+
+    Variant fulfill_step (tid:Id.t) (ts: Time.t) (eu1 eu2:t): Prop :=
+    | fulfill_step_intro
+        (STEP: ExecUnit.state_step tid eu1 eu2)
+        (FULFILL: fulfilled ts eu1 eu2)
+    .
+    #[local]
+     Hint Constructors fulfill_step: core.
 
     Lemma state_step0_wf tid e1 e2 eu1 eu2
           (STEP: state_step0 tid e1 e2 eu1 eu2)
@@ -169,7 +299,7 @@ Module PFRelExecUnit.
         + eapply fulfill_step_wf; try exact STEP_FULFILL; cycle 1.
           { inv STEP_PROMISE. inv MEM2.
             rewrite List.app_length; s.
-            rewrite <- TS1. erewrite expr_wf; eauto. lia.
+            rewrite <- TS1. erewrite expr_wf; eauto. nia.
           }
           eapply promise_wf; try exact PROMISE; eauto.
       - inv STEP. econs; ss. apply rmap_add_wf; viewtac.
@@ -219,6 +349,203 @@ Module PFRelExecUnit.
     Proof.
       inv STEP. eapply state_step0_wf; eauto. refl.
     Qed.
+
+    Lemma non_rel_step_wf tid eu1 eu2
+          (STEP: non_rel_step tid eu1 eu2)
+          (WF: wf tid eu1):
+      wf tid eu2.
+    Proof.
+      inv STEP. eapply ExecUnit.state_step0_wf; eauto. refl.
+    Qed.
+
+    Lemma rel_step_wf tid eu1 eu2
+          (STEP: rel_step tid eu1 eu2)
+          (WF: wf tid eu1):
+      wf tid eu2.
+    Proof.
+      inv STEP. eapply ExecUnit.state_step0_wf; eauto. refl.
+    Qed.
+
+    Lemma state_step0_promises_le
+          tid e1 e2 eu1 eu2
+          (STEP: state_step0 tid e1 e2 eu1 eu2):
+      Promises.le eu2.(local).(Local.promises) eu1.(local).(Local.promises).
+    Proof.
+      inv STEP. eauto using PFRelLocal.step_promises_le.
+    Qed.
+
+    Lemma state_step_promises_le
+          tid eu1 eu2
+          (STEP: state_step tid eu1 eu2):
+      Promises.le eu2.(local).(Local.promises) eu1.(local).(Local.promises).
+    Proof.
+      inv STEP. eauto using state_step0_promises_le.
+    Qed.
+
+    Lemma rtc_state_step_promises_le
+          tid eu1 eu2
+          (STEPS: rtc (state_step tid) eu1 eu2):
+      Promises.le eu2.(local).(Local.promises) eu1.(local).(Local.promises).
+    Proof.
+      induction STEPS; ss.
+      etrans; eauto using state_step_promises_le.
+    Qed.
+
+    Lemma non_rel_step_state_step
+          tid eu1 eu2
+          (STEP: non_rel_step tid eu1 eu2):
+      state_step tid eu1 eu2.
+    Proof.
+      inv STEP. inv STEP0.
+      econs. econs; eauto.
+      inv LOCAL; ss.
+      - econs 1; eauto.
+      - econs 2; eauto.
+      - econs 3; eauto.
+        destruct ord; ss.
+      - econs 5; eauto.
+      - econs 6; eauto.
+        destruct ordw; ss.
+      - econs 8; eauto.
+      - econs 9; eauto.
+        destruct rw, ww; ss.
+      - econs 10; eauto.
+    Qed.
+
+    Lemma fulfilled_dec ts eu1 eu2:
+      fulfilled ts eu1 eu2 \/ ~ fulfilled ts eu1 eu2.
+    Proof.
+      destruct (Promises.lookup ts eu1.(ExecUnit.local).(Local.promises)) eqn:LOOKUP1.
+      - destruct (Promises.lookup ts eu2.(ExecUnit.local).(Local.promises)) eqn:LOOKUP2.
+        + right. ii. inv H1.
+          rewrite LOOKUP1, LOOKUP2 in *. ss.
+        + left. econs; eauto. rewrite LOOKUP2. ss.
+      - right. ii. inv H1.
+        rewrite LOOKUP1 in *. ss.
+    Qed.
+
+    Lemma rtc_fulfilled_or
+          tid eu1 eu2 eu3 ts
+          (STEPS1: rtc (ExecUnit.state_step tid) eu1 eu2)
+          (STEPS2: rtc (ExecUnit.state_step tid) eu2 eu3)
+          (FULFILL: fulfilled ts eu1 eu3):
+      fulfilled ts eu1 eu2 \/ fulfilled ts eu2 eu3.
+    Proof.
+      revert eu3 STEPS2 FULFILL.
+      induction STEPS1; i; auto.
+      specialize (fulfilled_dec ts x y). i. des.
+      { left.
+        hexploit ExecUnit.rtc_state_step_promises_le; try exact STEPS1. i.
+        inv H2. econs; ss. ii.
+        apply H3 in H2. ss.
+      }
+      exploit IHSTEPS1; eauto.
+      { inv FULFILL. econs; ss.
+        destruct (Promises.lookup ts y.(local).(Local.promises)) eqn:LOOKUP; ss.
+        exfalso. apply H2. econs; ss.
+        rewrite LOOKUP. ss.
+      }
+      i. des; auto. left.
+      inv x1. econs; ss.
+      hexploit ExecUnit.state_step_promises_le; try exact H1. auto.
+    Qed.
+
+    Lemma or_rtc_fulfilled
+          tid eu1 eu2 eu3 ts
+          (STEPS1: rtc (ExecUnit.state_step tid) eu1 eu2)
+          (STEPS2: rtc (ExecUnit.state_step tid) eu2 eu3)
+          (FULFILL: fulfilled ts eu1 eu2 \/ fulfilled ts eu2 eu3):
+      fulfilled ts eu1 eu3.
+    Proof.
+      des.
+      - inv FULFILL. econs; ss. ii.
+        eapply ExecUnit.rtc_state_step_promises_le in H1; eauto.
+      - inv FULFILL. econs; ss.
+        eapply ExecUnit.rtc_state_step_promises_le in BEFORE; eauto.
+    Qed.
+
+    Lemma rtc_fulfilled_fulfill_step
+          tid eu1 eu4 ts
+          (STEPS: rtc (ExecUnit.state_step tid) eu1 eu4)
+          (FULFILL: fulfilled ts eu1 eu4):
+      exists eu2 eu3,
+        (<<STEPS1: rtc (ExecUnit.state_step tid) eu1 eu2>>) /\
+        (<<FULFILL: fulfill_step tid ts eu2 eu3>>) /\
+        (<<STEPS2: rtc (ExecUnit.state_step tid) eu3 eu4>>).
+    Proof.
+      induction STEPS.
+      { inv FULFILL. ss. }
+      exploit rtc_fulfilled_or; try exact FULFILL.
+      { econs 2; try refl. eauto. }
+      { ss. }
+      i. des; cycle 1.
+      { exploit IHSTEPS; eauto. i. des.
+        esplits; try exact FULFILL0; eauto.
+      }
+      esplits; [refl|..]; eauto.
+    Qed.
+
+    Variant more_promises (eu1 eu2: t): Prop :=
+    | more_promises_intro
+        (STATE: state eu1 = state eu2)
+        (LOCAL: PFRelLocal.more_promises (length (mem eu1)) (local eu1) (local eu2))
+        (MEMORY: exists mem_app, mem eu2 = mem eu1 ++ mem_app)
+    .
+
+    Global Program Instance more_promises_PreOrder: PreOrder more_promises.
+    Next Obligation.
+      ii. econs; ss; try refl.
+      exists []. rewrite List.app_nil_r. ss.
+    Qed.
+    Next Obligation.
+      ii. inv H1. inv H2. des.
+      econs; try congr.
+      - etrans; eauto.
+        eapply PFRelLocal.more_promises_decr; eauto.
+        rewrite MEMORY, app_length. nia.
+      - rewrite MEMORY0, MEMORY.
+        rewrite <- app_assoc.
+        esplits; eauto.
+    Qed.
+
+    Lemma promise_step_more_promises
+          tid eu1 eu2
+          (STEP: promise_step tid eu1 eu2):
+      more_promises eu1 eu2.
+    Proof.
+      destruct eu1, eu2.
+      inv STEP. inv LOCAL. inv MEM2. ss. subst.
+      econs; ss; eauto.
+      econs; ss.
+      - apply Promises.set_le.
+      - ii. rewrite Promises.set_o. condtac; ss.
+        rewrite e in *. nia.
+    Qed.
+
+    Lemma rtc_promise_step_more_promises
+          tid eu1 eu2
+          (STEPS: rtc (promise_step tid) eu1 eu2):
+      more_promises eu1 eu2.
+    Proof.
+      induction STEPS; try refl.
+      etrans; eauto.
+      eapply promise_step_more_promises; eauto.
+    Qed.
+
+    Lemma more_promises_app
+          eu1 eu2 eu1'
+          (MORE: more_promises eu1 eu2)
+          (STATE: state eu1 = state eu1')
+          (LOCAL: local eu1 = local eu1')
+          (MEMORY: exists mem_app, mem eu1 = mem eu1' ++ mem_app):
+      more_promises eu1' eu2.
+    Proof.
+      destruct eu1, eu2, eu1'. inv MORE. ss. des. subst.
+      econs; ss.
+      - eapply PFRelLocal.more_promises_decr; eauto.
+        rewrite app_length. nia.
+      - rewrite <- app_assoc. eauto.
+    Qed.
   End PFRelExecUnit.
 End PFRelExecUnit.
 
@@ -233,6 +560,38 @@ Module PFRelMachine.
   .
   #[global]
    Hint Constructors exec: core.
+
+  Lemma rtc_promise_step_more_promises
+        m1 m2
+        (STEPS: rtc (step ExecUnit.promise_step) m1 m2):
+    IdMap.Forall2
+      (fun tid sl1 sl2 =>
+         PFRelExecUnit.more_promises
+           (ExecUnit.mk (fst sl1) (snd sl1) m1.(mem))
+           (ExecUnit.mk (fst sl2) (snd sl2) m2.(mem)))
+      m1.(tpool) m2.(tpool).
+  Proof.
+    induction STEPS; ii.
+    { destruct (IdMap.find id (tpool x)); ss. econs. refl. }
+    inv H.
+    specialize (IHSTEPS id). revert IHSTEPS.
+    destruct (IdMap.find id (tpool x)) eqn:FINDx.
+    { rewrite TPOOL, IdMap.add_spec. condtac.
+      - inversion e. subst.
+        rewrite FIND in *. inv FINDx.
+        exploit (@PFRelExecUnit.promise_step_more_promises unit); eauto. i.
+        inv IHSTEPS. ss.
+        econs. etrans; eauto.
+      - rewrite FINDx. i. inv IHSTEPS.
+        econs. ss.
+        eapply PFRelExecUnit.more_promises_app; try exact REL; eauto.
+        inv STEP. inv LOCAL. inv MEM2. ss. eauto.
+    }
+    { rewrite TPOOL, IdMap.add_spec. condtac.
+      { inversion e. subst. congr. }
+      rewrite FINDx. i. inv IHSTEPS. econs.
+    }
+  Qed.
 
   Variant pf_rel_until_eu (tid: Id.t) (n: nat) (eu1 eu2: ExecUnit.t (A:=unit)): Prop :=
   | pf_re_until_eu_intro
@@ -276,10 +635,17 @@ Module PFRelMachine.
     - inv STEP2. ii.
       specialize (TPOOL id). inv TPOOL; eauto.
       econs. econs; eauto. ss.
-      admit.
+      hexploit rtc_promise_step_more_promises; eauto. i.
+      specialize (H1 id).
+      rewrite <- H0 in *. inv H1.
+      revert H3. rewrite IdMap.map_spec.
+      destruct (IdMap.find id p); ss. i. inv H3. ss.
+      inv REL0. ss. inv LOCAL.
+      destruct ts; try nia.
+      exploit PROMISES_EQ; try refl. ss.
     - inv STEP2. ss.
     - ss.
-  Admitted.
+  Qed.
 
   Lemma pf_rel_until_step
         n m_init m_final
@@ -288,7 +654,7 @@ Module PFRelMachine.
     pf_rel_until (S n) m_init m_final.
   Proof.
     inv UNTIL. inv PROMISES.
-    { rewrite MEMORY in *. lia. }
+    { rewrite MEMORY in *. nia. }
     rename y into m. inv H.
     dup STATE_EXEC.
   Admitted.
